theories/geuvers.v
@@ -1,0 +1,84 @@
+Require Export typing.
+
+Inductive kind_interp Γ : Term -> Type -> Prop :=
+| KI_Star :
+  kind_interp Γ (ISort Star) (Term -> Prop)
+| KI_Imp A B S0 S1 :
+  kind_interp Γ A S0 ->
+  kind_interp (A::Γ) B S1 ->
+  kind_interp Γ (Pi A B) (S0 -> S1 -> Prop)
+| KI_Fun A B S :
+  Γ ⊢ A ∈ ISort Star ->
+  kind_interp (A::Γ) B S ->
+  kind_interp Γ (Pi A B) S.
+
+(* Lemma that gives the shape of a kind (excludes app) *)
+
+(* Lemma subject_reduction Γ a A  : *)
+(*   Γ ⊢ a ∈ A -> forall b, a ⇒ b -> Γ ⊢ b ∈ A. *)
+(* Proof. Admitted. *)
+
+(* Lemma kind_interp_eval Γ A B S : *)
+(*   kind_interp Γ A S -> A ⇒ B -> kind_interp Γ B S. *)
+(* Proof. *)
+(*   move => h. move : B. elim : Γ A S /h. *)
+(*   - hauto l:on inv:Par. *)
+(*   - move => Γ A B S0 S1 hA ihA hB ihB. *)
+(*     admit. *)
+(* Admitted. *)
+
+Lemma kind_imp Γ A :
+  ~ Γ ⊢ ISort Kind ∈ A.
+Proof.
+  move E : (ISort Kind) => a h.
+  move : E.
+  elim : Γ a A /h=>//=.
+Qed.
+
+Lemma wt_has_interp Γ A :
+  Γ ⊢ A ∈ ISort Kind -> exists V, kind_interp Γ A V.
+Proof.
+  move E : (ISort Kind) => U h.
+  move : E.
+  elim : Γ A U /h=>//=.
+  - move => Γ i A h ?. subst.
+    (* Impossible because Kind doesn't have a sort *)
+    admit.
+  - eauto using KI_Star.
+  - move => Γ a b A B ha _ hb _ E.
+    have : Γ ⊢ App b a ∈ B[a…] by  eauto using T_App.
+    (* Contradiction *)
+    admit.
+  - move => Γ A s1 B s2 hA ihA hB ihB [?]. subst.
+    specialize ihB with (1 := eq_refl).
+    case : s1 hA ihA; hauto lq:on ctrs:kind_interp.
+  - (* Impossible *)
+    move => Γ a A B s ha iha hB ihB heq ?. subst.
+    firstorder using kind_imp.
+Admitted.
+
+Lemma kind_interp_not_star Γ A S :
+  kind_interp Γ A S ->
+  ~ Γ ⊢ A ∈ ISort Star.
+Proof.
+  move => h. elim : Γ A S /h.
+  - admit.
+  - move => Γ A B S0 S1 hA ihA hB ihB.
+    admit.
+  - move => Γ A B S hA ihA hB h.
+Admitted.
+
+Lemma kind_interp_functionality Γ A S0 S1 :
+  kind_interp Γ A S0 -> kind_interp Γ A S1 -> S0 = S1.
+Proof.
+  move => h. move : S1. elim : Γ A S0 / h.
+  - hauto lq:on inv:kind_interp.
+  - move => Γ A B SA0 SB0 hA ihA hB ihB S.
+    inversion 1; subst.
+    sfirstorder.
+    firstorder using kind_interp_not_star.
+  - move => Γ A B S hA ihA hB S0.
+    inversion 1.
+    by firstorder using kind_interp_not_star.
+    sfirstorder.
+Qed.
